Use positive integer instead of natural for type of ReprDepth

src/linear/layer1/ADT.dfy
@@ -1,5 +1,7 @@
+type pos = n: int | n > 0 witness 1
+
 trait ADT<M> {
-  ghost const ReprDepth: nat
+  ghost const ReprDepth: pos
 
   function ReprFamily(n: nat): set<object>
     decreases n
@@ -7,7 +9,7 @@ trait ADT<M> {
     reads this, if n == 0 then {} else ReprFamily(n-1)
 
   function Repr(): set<object>
-    reads this, if ReprDepth == 0 then {} else ReprFamily(ReprDepth-1)
+    reads this, ReprFamily(ReprDepth-1)
   {
     ReprFamily(ReprDepth)
   }
